Ported revisions 8163:8176 from HOL to HOL-Omega. This is to keep HOL-Omega current with the latest HOL developments.

developers/generateBuildSummary.sml
@@ -1,0 +1,43 @@
+structure generateBuildSummary =
+struct
+
+(* reads the output of bin/build on standard input, and turns it into a
+   mail message *)
+
+fun datestring t = let
+  open Date
+in
+  fmt "%a, %d %b %Y %H:%M UT" (fromTimeUniv t)
+end
+
+fun standard_header from subject t =
+    "To: hol-builds@lists.sourceforge.net\n\
+    \From: "^from^"\n\
+    \Date: "^datestring t^"\n\
+    \Subject: "^subject^"\n\n"
+
+fun usage() =
+    (TextIO.output(TextIO.stdErr,
+                   "Usage:\n  "^CommandLine.name()^
+                   " from-address system-description\n");
+     TextIO.flushOut TextIO.stdErr;
+     OS.Process.exit OS.Process.failure)
+
+fun main() = let
+  val (from, sysdesc) = case CommandLine.arguments() of
+               [f,s] => (f,s)
+             | _ => usage()
+  val buildlog = TextIO.inputAll TextIO.stdIn
+  open TextIO
+in
+  if String.isSuffix "Hol built successfully.\n" buildlog then
+    output(stdOut,
+           standard_header from ("SUCCESS: "^sysdesc) (Time.now()) ^
+           buildlog)
+  else
+    output(stdOut,
+           standard_header from ("FAILURE: "^sysdesc) (Time.now()) ^
+           buildlog)
+end
+
+end
