examples/separationLogic/src/holfoot/Parsetree.sml
@@ -59,11 +59,12 @@ datatype p_statement =
   | Pstm_dispose of a_expression * a_expression
   | Pstm_block of p_statement list
   | Pstm_if of p_condition * p_statement * p_statement
-  | Pstm_while of read_write_decl * a_invariant * p_condition * p_statement
-  | Pstm_block_spec of bool * read_write_decl * a_proposition * p_statement * a_proposition
+  | Pstm_while of int * read_write_decl * a_invariant * p_condition * p_statement
+  | Pstm_block_spec of bool * int * read_write_decl * a_proposition * p_statement * a_proposition
   | Pstm_withres of string * p_condition * p_statement
   | Pstm_fcall of string * actual_params
   | Pstm_parallel_fcall of string * actual_params * string * actual_params
+  | Pstm_assert of a_proposition
 
 
 datatype p_item =
